fv/lean/Ragu/Circuits/Element/Mul.lean
@@ -3,19 +3,18 @@ import Ragu.Circuits.Core.AllocMul
 
 namespace Ragu.Circuits.Element.Mul
 variable {p : ℕ} [Fact p.Prime]
-variable {ProverHint : Type}
 
 structure Input (F : Type) where
   x : F
   y : F
 deriving ProvableStruct
 
-def main (input : Var Input (F p)) : Circuit (F p) ProverHint (Var field (F p)) := do
+def main (input : Var Input (F p)) : Circuit (F p) (Var field (F p)) := do
   let ⟨x, y, z⟩ ← (witness fun env _hint =>
     let xv := Expression.eval env input.x
     let yv := Expression.eval env input.y
     ⟨xv, yv, xv * yv⟩
-    : Circuit (F p) ProverHint (Var Core.AllocMul.Row (F p)))
+    : Circuit (F p) (Var Core.AllocMul.Row (F p)))
   assertZero (x * y - z)
   assertZero (x - input.x)
   assertZero (y - input.y)
@@ -26,17 +25,17 @@ def Assumptions (_input : Input (F p)) := True
 def Spec (input : Input (F p)) (out : field (F p)) :=
   out = input.x * input.y
 
-instance elaborated : ElaboratedCircuit (F p) ProverHint Input field where
+instance elaborated : ElaboratedCircuit (F p) Input field where
   main
   localLength _ := 3
 
-theorem soundness : Soundness (F p) ProverHint elaborated Assumptions Spec := by
+theorem soundness : Soundness (F p) elaborated Assumptions Spec := by
   circuit_proof_start
   obtain ⟨c1, c2, c3⟩ := h_holds
   rw [add_neg_eq_zero] at c1 c2 c3
   rw [←c2, ←c3, c1]
 
-theorem completeness : Completeness (F p) ProverHint elaborated Assumptions := by
+theorem completeness : Completeness (F p) elaborated Assumptions := by
   circuit_proof_start
   have h0 := h_env (0 : Fin 3)
   have h1 := h_env (1 : Fin 3)
@@ -48,7 +47,7 @@ theorem completeness : Completeness (F p) ProverHint elaborated Assumptions := b
   rw [h0, h1, h2]
   refine ⟨?_, ?_, ?_⟩ <;> ring
 
-def circuit : FormalCircuit (F p) ProverHint Input field :=
+def circuit : FormalCircuit (F p) Input field :=
   { elaborated with Assumptions, Spec, soundness, completeness }
 
 end Ragu.Circuits.Element.Mul
