fv/lean/Ragu/Circuits/Point/AddIncomplete.lean
@@ -20,14 +20,14 @@ structure Outputs (F : Type) where
   nonzero : F
 deriving ProvableStruct
 
-def main (input : Var Inputs (F p)) : Circuit (F p) (Core.AllocMul.Row (F p)) (Var Outputs (F p)) := do
+def main (idx : ℕ) (input : Var Inputs (F p)) : Circuit (F p) (Var Outputs (F p)) := do
   let ⟨⟨x1, y1⟩, ⟨x2, y2⟩, nonzero⟩ := input
 
   -- delta = (y2 - y1) / (x2 - x1)
   let tmp := x2 - x1
   let nonzero_out ← subcircuit Element.Mul.circuit ⟨nonzero, tmp⟩
 
-  let delta ← Element.DivNonzero.generalCircuit ⟨y2 - y1, tmp⟩
+  let delta ← Element.DivNonzero.generalCircuit idx ⟨y2 - y1, tmp⟩
 
   -- x3 = delta^2 - x1 - x2
   let ⟨delta2⟩ ← subcircuit Element.Square.circuit ⟨delta⟩
@@ -42,45 +42,38 @@ def main (input : Var Inputs (F p)) : Circuit (F p) (Core.AllocMul.Row (F p)) (V
     nonzero := nonzero_out
   }
 
-def Assumptions (curveParams : Spec.CurveParams p)
-    (input : Inputs (F p)) (data : ProverData (F p)) (hint : Core.AllocMul.Row (F p)) :=
+def Assumptions (curveParams : Spec.CurveParams p) (idx : ℕ)
+    (input : Inputs (F p)) (data : ProverData (F p)) (hint : ProverHint (F p)) :=
   input.P1.isOnCurve curveParams ∧ input.P2.isOnCurve curveParams ∧
-  Element.DivNonzero.GeneralAssumptions ⟨input.P2.y - input.P1.y, input.P2.x - input.P1.x⟩ data hint
+  Element.DivNonzero.GeneralAssumptions idx ⟨input.P2.y - input.P1.y, input.P2.x - input.P1.x⟩ data hint
 
 def Spec (curveParams : Spec.CurveParams p) (input : Inputs (F p)) (output : Outputs (F p)) (_data : ProverData (F p)) :=
   input.P1.isOnCurve curveParams →
   input.P2.isOnCurve curveParams →
   (
-    -- If the x coordinates of P1 and P2 are different, then we can conclude that the
-    -- addition output is affine and is the correct result of the addition
     input.P1.x ≠ input.P2.x -> (
       (
         match input.P1.add_incomplete input.P2  with
-        | none => False -- this case never happens
+        | none => False
         | some res => output.P3 = res
       )
       ∧ output.P3.isOnCurve curveParams
     )
   ) ∧
   (
-    -- if the x coordinates of P1 and P2 are equal, then output nonzero is 0
-    -- regardless of the input nonzero
     (input.P1.x = input.P2.x -> output.nonzero = 0) ∧
-
-    -- if the x coordinates of P1 and P2 are not equal, then output nonzero preserves
-    -- non-zero-ness from input nonzero
     (input.P1.x ≠ input.P2.x ->
       (input.nonzero = 0 -> output.nonzero = 0) ∧
       (input.nonzero ≠ 0 -> output.nonzero ≠ 0)
     )
   )
 
-instance elaborated : ElaboratedCircuit (F p) (Core.AllocMul.Row (F p)) Inputs Outputs where
-  main
+instance elaborated (idx : ℕ) : ElaboratedCircuit (F p) Inputs Outputs where
+  main := main idx
   localLength _ := 12
 
-theorem soundness (curveParams : Spec.CurveParams p) :
-    GeneralFormalCircuit.Soundness (F p) (Core.AllocMul.Row (F p)) elaborated (Spec curveParams) := by
+theorem soundness (curveParams : Spec.CurveParams p) (idx : ℕ) :
+    GeneralFormalCircuit.Soundness (F p) (elaborated idx) (Spec curveParams) := by
   circuit_proof_start
   simp [circuit_norm,
     Element.Square.circuit, Element.Square.Assumptions, Element.Square.Spec,
@@ -116,8 +109,8 @@ theorem soundness (curveParams : Spec.CurveParams p) :
     apply Ne.symm
     exact h1
 
-theorem completeness (curveParams : Spec.CurveParams p) :
-    GeneralFormalCircuit.Completeness (F p) (Core.AllocMul.Row (F p)) elaborated (Assumptions curveParams) := by
+theorem completeness (curveParams : Spec.CurveParams p) (idx : ℕ) :
+    GeneralFormalCircuit.Completeness (F p) (elaborated idx) (Assumptions curveParams idx) := by
   circuit_proof_start [
     Element.Square.circuit, Element.Square.Assumptions,
     Element.DivNonzero.generalCircuit, Element.DivNonzero.GeneralAssumptions,
@@ -126,14 +119,14 @@ theorem completeness (curveParams : Spec.CurveParams p) :
   simp only [sub_eq_add_neg] at h_assumptions
   exact h_assumptions.2.2
 
-def circuit (curveParams : Spec.CurveParams p) :
-    GeneralFormalCircuit (F p) (Core.AllocMul.Row (F p)) Inputs Outputs :=
+def circuit (curveParams : Spec.CurveParams p) (idx : ℕ) :
+    GeneralFormalCircuit (F p) Inputs Outputs :=
   {
-    elaborated with
-    Assumptions := Assumptions curveParams,
+    elaborated idx with
+    Assumptions := Assumptions curveParams idx,
     Spec := Spec curveParams,
-    soundness := soundness curveParams,
-    completeness := completeness curveParams
+    soundness := soundness curveParams idx,
+    completeness := completeness curveParams idx
   }
 
 end Ragu.Circuits.Point.AddIncomplete
